remove axioms

DistributedSystems/VerifiedDS/src/Dafny/Distributed/Protocol/CausalMesh/message.dfy
@@ -7,10 +7,10 @@ module CausalMesh_Message_i {
 
     datatype Message = 
         //   Message_Invalid()
-          Message_Read(opn_read:int, key_read:Key, deps_read:Dependency)
-        | Message_Read_Reply(opn_rreply:int, key_rreply:Key, vc_rreply:VectorClock, deps_rreply:Dependency)
-        | Message_Write(opn_write:int, key_write:Key, deps_write:Dependency, local:map<Key, Meta>)
-        | Message_Write_Reply(opn_wreply:int, key_wreply:Key, vc_wreply:VectorClock)
+          Message_Read(opn_read:int, key_read:Key, deps_read:Dependency, pvc_read:VectorClock)
+        | Message_Read_Reply(opn_rreply:int, key_rreply:Key, vc_rreply:VectorClock, deps_rreply:Dependency, pvc_rreply:VectorClock)
+        | Message_Write(opn_write:int, key_write:Key, deps_write:Dependency, local:map<Key, Meta>, pvc_write:VectorClock)
+        | Message_Write_Reply(opn_wreply:int, key_wreply:Key, vc_wreply:VectorClock, pvc_wreply:VectorClock)
         // | Message_Propagation(key:Key, metas:set<Meta>, start:int)
         | Message_Propagation(key:Key, meta:Meta, start:int, round:int)
 
@@ -18,10 +18,10 @@ module CausalMesh_Message_i {
     {
         match m 
             // case Message_Invalid() => true
-            case Message_Read(_,key_read, deps_read) => key_read in Keys_domain && DependencyValid(deps_read)
-            case Message_Read_Reply(_,key_rreply, vc_rreply, deps_rreply) => key_rreply in Keys_domain && VectorClockValid(vc_rreply) && DependencyValid(deps_rreply)
-            case Message_Write(_,key_write, deps_write, local) => key_write in Keys_domain && DependencyValid(deps_write) && (forall k :: k in local ==> MetaValid(local[k]))
-            case Message_Write_Reply(_,key_wreply, vc_wreply/*, deps_wreply*/) => key_wreply in Keys_domain && VectorClockValid(vc_wreply) // && DependencyValid(deps_wreply)
+            case Message_Read(_,key_read, deps_read, gvc_read) => key_read in Keys_domain && DependencyValid(deps_read) && VectorClockValid(gvc_read)
+            case Message_Read_Reply(_,key_rreply, vc_rreply, deps_rreply, gvc_rreply) => key_rreply in Keys_domain && VectorClockValid(vc_rreply) && DependencyValid(deps_rreply) && VectorClockValid(gvc_rreply)
+            case Message_Write(_,key_write, deps_write, local, gvc_write) => key_write in Keys_domain && DependencyValid(deps_write) && (forall k :: k in local ==> MetaValid(local[k])) && VectorClockValid(gvc_write)
+            case Message_Write_Reply(_,key_wreply, vc_wreply, pvc_wreply/*, deps_wreply*/) => key_wreply in Keys_domain && VectorClockValid(vc_wreply) && VectorClockValid(pvc_wreply) // && DependencyValid(deps_wreply)
             case Message_Propagation(key, meta, start, round) => key in Keys_domain && (MetaValid(meta) && meta.key == key) && 0 <= start < Nodes
     }
 
@@ -38,10 +38,10 @@ module CausalMesh_Message_i {
     predicate PacketHasCorrectSrcAndDst(p:Packet)
     {
         match p.msg 
-            case Message_Read(_,_,_) => Nodes <= p.src < Nodes + Clients && 0 <= p.dst < Nodes
-            case Message_Read_Reply(_,_,_,_) => Nodes <= p.dst < Nodes + Clients && 0 <= p.src < Nodes
-            case Message_Write(_,_,_,_) => Nodes <= p.src < Nodes + Clients && 0 <= p.dst < Nodes
-            case Message_Write_Reply(_,_,_) => Nodes <= p.dst < Nodes + Clients && 0 <= p.src < Nodes
+            case Message_Read(_,_,_,_) => Nodes <= p.src < Nodes + Clients && 0 <= p.dst < Nodes
+            case Message_Read_Reply(_,_,_,_,_) => Nodes <= p.dst < Nodes + Clients && 0 <= p.src < Nodes
+            case Message_Write(_,_,_,_,_) => Nodes <= p.src < Nodes + Clients && 0 <= p.dst < Nodes
+            case Message_Write_Reply(_,_,_,_) => Nodes <= p.dst < Nodes + Clients && 0 <= p.src < Nodes
             case Message_Propagation(_,_,_,_) => 0 <= p.src < Nodes && 0 <= p.dst < Nodes && NodesAreNext(p.src, p.dst)
     }
 }
