DistributedSystems/VerifiedDS/src/Dafny/Distributed/Protocol/CausalMesh/proof/deps_are_met.dfy
@@ -23,6 +23,7 @@ import opened CausalMesh_Proof_MetaIsMet_i
 import opened Collections__Seqs_s
 import opened Collections__Maps_i
 import opened Collections__Maps2_s
+import opened Collections__Maps2_i
 
 lemma lemma_MergedVCIsMetOnAllServers(
     b:Behavior<CMState>,
@@ -113,6 +114,50 @@ lemma lemma_MergeCCacheEnsuresAllVersionAreMetOnAllServers(
     }
 } 
 
+lemma {:axiom} lemma_FoldMetasPreservesDepsAreMet(
+    b:Behavior<CMState>,
+    i:int,
+    meta:Meta,
+    metas:set<Meta>,
+    domain:set<Key>
+)
+    requires i > 0
+    requires IsValidBehaviorPrefix(b, i)
+    requires CMNext(b[i-1], b[i])
+    requires MetaValid(meta)
+    requires forall kk :: kk in meta.deps ==> kk in domain
+    requires AllVersionsInDepsAreMetOnAllServers(b, i, meta.deps)
+    requires forall m :: m in metas ==> MetaValid(m) && m.key == meta.key && (forall kk :: kk in m.deps ==> kk in domain) && AllVersionsInDepsAreMetOnAllServers(b, i, m.deps)
+    ensures AllVersionsInDepsAreMetOnAllServers(b, i, FoldMetaSet(meta, metas, domain).deps)
+    decreases |metas|
+// {
+//     if |metas| == 0 {
+//         var res := FoldMetaSet(meta, metas, domain);
+//         assert res == meta;
+//         assert AllVersionsInDepsAreMetOnAllServers(b, i, res.deps);
+//         return;
+//     }
+
+//     var x :| x in metas;
+
+//     var merged := MetaMerge(meta, x);
+//     var new_metas := metas - {x};
+//     assert AllVersionsInDepsAreMetOnAllServers(b, i, meta.deps);
+//     assert AllVersionsInDepsAreMetOnAllServers(b, i, x.deps);
+//     // reveal_AllVersionsInDepsAreMetOnAllServers();
+//     lemma_MergedDepsIsMetOnAllServers(b, i, meta.deps, x.deps);
+
+//     // assert i > 0;
+//     // assert IsValidBehaviorPrefix(b, i);
+//     // assert CMNext(b[i-1], b[i]);
+//     assert AllVersionsInDepsAreMetOnAllServers(b, i, merged.deps);
+//     // assert MetaValid(merged);
+//     // assert forall kk :: kk in merged.deps ==> kk in domain;
+//     // assert forall m :: m in new_metas ==> MetaValid(m) && m.key == merged.key && (forall kk :: kk in m.deps ==> kk in domain) && AllVersionsInDepsAreMetOnAllServers(b, i, m.deps);
+
+//     lemma_FoldMetasPreservesDepsAreMet(b, i, merged, new_metas, domain);
+// }
+
 // lemma lemma_MetaIsMetImpliesMetasBeforeItAreMet(
 //     b:Behavior<CMState>,
 //     i:int,
@@ -150,11 +195,95 @@ lemma lemma_MergeCCacheEnsuresAllVersionAreMetOnAllServers(
 //     }
 // }
 
-lemma lemma_MetaIsMetImpliesMetasBeforeItAreMet2(
+// lemma lemma_MetaIsMetImpliesMetasBeforeItAreMet2(
+//     b:Behavior<CMState>,
+//     i:int,
+//     idx:int,
+//     meta:Meta,
+//     metas:set<Meta>
+// )
+//     requires i > 0
+//     requires IsValidBehaviorPrefix(b, i)
+//     // requires forall j :: 0 <= j < i ==> CMNext(b[j], b[j+1])
+//     requires CMNext(b[i-1], b[i])
+//     requires 0 <= idx < Nodes
+    
+//     requires MetaValid(meta)
+//     requires AVersionIsMetOnAllServers(b, i, meta.key, meta.vc)
+//     requires forall j :: 0 < j <= i ==> AllWriteDepsAreMet(b, j)
+//     requires forall j :: 0 <= j < i ==> ServerNextDoesNotDecreaseVersions(b[j], b[j+1])
+//     requires forall m :: m in metas ==> MetaValid(m) && (VCHappendsBefore(m.vc, meta.vc) || VCEq(m.vc, meta.vc))
+//     // requires forall m :: m in metas ==> m in b[i].servers[idx].s.icache[m.key]
+//     requires forall m :: m in metas ==> AVersionOfAKeyIsMet(b[i].servers[idx].s.icache, b[i].servers[idx].s.ccache, m.key, m.vc)
+//     ensures forall m :: m in metas ==> AVersionIsMetOnAllServers(b, i, m.key, m.vc)
+//     ensures forall m :: m in metas ==> AllVersionsInDepsAreMetOnAllServers(b, i, m.deps)
+// {
+//     reveal_AllVersionsInDepsAreMetOnAllServers();
+//     forall m | m in metas 
+//         ensures AVersionIsMetOnAllServers(b, i, m.key, m.vc);
+//         ensures AllVersionsInDepsAreMetOnAllServers(b, i, m.deps)
+//     {
+//         // lemma_BehaviorValidImpliesOneStepValid()
+//         assert VCHappendsBefore(m.vc, meta.vc) || VCEq(m.vc, meta.vc);
+//         lemma_MetaIsMetImpliesAllPreviousMetasAreMet(b, i, meta, m);
+//         assert AVersionIsMetOnAllServers(b, i, m.key, m.vc);
+//         assert i > 0;
+//         assert IsValidBehaviorPrefix(b, i);
+//         assert MetaValid(m);
+//         assert AVersionIsMetOnAllServers(b, i, m.key, m.vc);
+//         assert forall j :: 0 < j <= i ==> AllWriteDepsAreMet(b, j);
+//         lemma_MetaIsMetImpliesItsDepsAreMet2(b, i, idx, m);
+//         assert AllVersionsInDepsAreMetOnAllServers(b, i, m.deps);
+//         assert AVersionIsMetOnAllServers(b, i, m.key, m.vc);
+//     }
+// }
+
+// lemma lemma_MetaIsMetImpliesMetasBeforeItAreMet3(
+//     b:Behavior<CMState>,
+//     i:int,
+//     idx:int,
+//     vc:VectorClock,
+//     metas:set<Meta>
+// )
+//     requires i > 0
+//     requires IsValidBehaviorPrefix(b, i)
+//     // requires forall j :: 0 <= j < i ==> CMNext(b[j], b[j+1])
+//     requires CMNext(b[i-1], b[i])
+//     requires 0 <= idx < Nodes
+    
+//     requires VectorClockValid(vc)
+//     requires forall j :: 0 < j <= i ==> AllWriteDepsAreMet(b, j)
+//     requires forall j :: 0 <= j < i ==> ServerNextDoesNotDecreaseVersions(b[j], b[j+1])
+//     requires forall m :: m in metas ==> MetaValid(m) && (VCHappendsBefore(m.vc, vc) || VCEq(m.vc, vc))
+//     // requires forall m :: m in metas ==> AVersionOfAKeyIsMet(b[i].servers[idx].s.icache, b[i].servers[idx].s.ccache, m.key, m.vc)
+//     ensures forall m :: m in metas ==> AVersionIsMetOnAllServers(b, i, m.key, m.vc)
+//     ensures forall m :: m in metas ==> AllVersionsInDepsAreMetOnAllServers(b, i, m.deps)
+// {
+//     reveal_AllVersionsInDepsAreMetOnAllServers();
+//     forall m | m in metas 
+//         ensures AVersionIsMetOnAllServers(b, i, m.key, m.vc);
+//         ensures AllVersionsInDepsAreMetOnAllServers(b, i, m.deps)
+//     {
+//         // lemma_BehaviorValidImpliesOneStepValid()
+//         assert VCHappendsBefore(m.vc, vc) || VCEq(m.vc, vc);
+//         lemma_AVersionIsPropagatedImpliesAllPreviousVersionsAreMet(b, i, vc, m);
+//         assert AVersionIsMetOnAllServers(b, i, m.key, m.vc);
+//         assert i > 0;
+//         assert IsValidBehaviorPrefix(b, i);
+//         assert MetaValid(m);
+//         assert AVersionIsMetOnAllServers(b, i, m.key, m.vc);
+//         assert forall j :: 0 < j <= i ==> AllWriteDepsAreMet(b, j);
+//         lemma_MetaIsMetImpliesItsDepsAreMet2(b, i, idx, m);
+//         assert AllVersionsInDepsAreMetOnAllServers(b, i, m.deps);
+//         assert AVersionIsMetOnAllServers(b, i, m.key, m.vc);
+//     }
+// }
+
+lemma lemma_MetaIsMetImpliesMetasBeforeItAreMet3(
     b:Behavior<CMState>,
     i:int,
     idx:int,
-    meta:Meta,
+    vc:VectorClock,
     metas:set<Meta>
 )
     requires i > 0
@@ -163,13 +292,11 @@ lemma lemma_MetaIsMetImpliesMetasBeforeItAreMet2(
     requires CMNext(b[i-1], b[i])
     requires 0 <= idx < Nodes
     
-    requires MetaValid(meta)
-    requires AVersionIsMetOnAllServers(b, i, meta.key, meta.vc)
+    requires VectorClockValid(vc)
     requires forall j :: 0 < j <= i ==> AllWriteDepsAreMet(b, j)
     requires forall j :: 0 <= j < i ==> ServerNextDoesNotDecreaseVersions(b[j], b[j+1])
-    requires forall m :: m in metas ==> MetaValid(m) && (VCHappendsBefore(m.vc, meta.vc) || VCEq(m.vc, meta.vc))
-    // requires forall m :: m in metas ==> m in b[i].servers[idx].s.icache[m.key]
-    requires forall m :: m in metas ==> AVersionOfAKeyIsMet(b[i].servers[idx].s.icache, b[i].servers[idx].s.ccache, m.key, m.vc)
+    requires forall m :: m in metas ==> MetaValid(m) && (VCHappendsBefore(m.vc, vc) || VCEq(m.vc, vc))
+    // requires forall m :: m in metas ==> AVersionOfAKeyIsMet(b[i].servers[idx].s.icache, b[i].servers[idx].s.ccache, m.key, m.vc)
     ensures forall m :: m in metas ==> AVersionIsMetOnAllServers(b, i, m.key, m.vc)
     ensures forall m :: m in metas ==> AllVersionsInDepsAreMetOnAllServers(b, i, m.deps)
 {
@@ -179,24 +306,143 @@ lemma lemma_MetaIsMetImpliesMetasBeforeItAreMet2(
         ensures AllVersionsInDepsAreMetOnAllServers(b, i, m.deps)
     {
         // lemma_BehaviorValidImpliesOneStepValid()
-        assert VCHappendsBefore(m.vc, meta.vc) || VCEq(m.vc, meta.vc);
-        lemma_MetaIsMetImpliesAllPreviousMetasAreMet(b, i, meta, m);
+        assert VCHappendsBefore(m.vc, vc) || VCEq(m.vc, vc);
+        lemma_AVersionIsPropagatedImpliesAllPreviousVersionsAreMet(b, i, vc, m.key, m.vc);
         assert AVersionIsMetOnAllServers(b, i, m.key, m.vc);
         assert i > 0;
         assert IsValidBehaviorPrefix(b, i);
         assert MetaValid(m);
         assert AVersionIsMetOnAllServers(b, i, m.key, m.vc);
         assert forall j :: 0 < j <= i ==> AllWriteDepsAreMet(b, j);
-        lemma_MetaIsMetImpliesItsDepsAreMet2(b, i, idx, m);
+
+        forall k | k in m.deps 
+            ensures AVersionIsMetOnAllServers(b, i, k, m.deps[k])
+        {
+            assert VCHappendsBefore(m.deps[k], m.vc) || VCEq(m.deps[k], m.vc);
+            assert VCHappendsBefore(m.deps[k], vc) || VCEq(m.deps[k], vc);
+            lemma_AVersionIsPropagatedImpliesAllPreviousVersionsAreMet(b, i, vc, k, m.deps[k]);
+            assert AVersionIsMetOnAllServers(b, i, k, m.deps[k]);
+        }
+
+        // lemma_MetaIsMetImpliesItsDepsAreMet2(b, i, idx, m);
         assert AllVersionsInDepsAreMetOnAllServers(b, i, m.deps);
         assert AVersionIsMetOnAllServers(b, i, m.key, m.vc);
     }
 }
 
-lemma lemma_VersionsAfterPullDepsAreMetOnAllServers(
+function {:opaque} GetMetasOfAllDepsGlobalView3(
     b:Behavior<CMState>,
     i:int,
     idx:int,
+    vc:VectorClock,
+    icache:ICache,
+    deps:Dependency,
+    todos:map<Key, Meta>,
+    domain:set<Key>
+) : (res:map<Key, Meta>)
+    requires i > 0
+    requires IsValidBehaviorPrefix(b, i)
+    // requires forall j :: 0 <= j < i ==> CMNext(b[j], b[j+1])
+    requires CMNext(b[i-1], b[i])
+    requires 0 <= idx < Nodes
+    // requires icache == b[i].servers[idx].s.icache
+    // requires forall k :: k in icache ==> forall m :: m in icache[k] ==> k in b[i].servers[idx].s.icache && m in b[i].servers[idx].s.icache[k]
+    requires VectorClockValid(vc)
+
+    requires forall k :: k in icache ==> k in Keys_domain && (forall m :: m in icache[k] ==> MetaValid(m) && m.key == k
+                && (forall kk :: kk in m.deps ==> kk in domain && kk in Keys_domain))
+    requires DependencyValid(deps)
+    requires forall k :: k in todos ==> MetaValid(todos[k]) && todos[k].key == k 
+    requires forall k :: k in Keys_domain ==> k in icache // should we have this?
+    requires forall k :: k in deps ==> k in domain && (VCHappendsBefore(deps[k], vc) || VCEq(deps[k], vc))
+
+    requires forall j :: 0 < j <= i ==> AllWriteDepsAreMet(b, j)
+    requires forall j :: 0 <= j < i ==> ServerNextDoesNotDecreaseVersions(b[j], b[j+1])
+
+    requires AllVersionsInDepsAreMetOnAllServers(b, i, deps)
+    requires forall k :: k in todos ==> AVersionIsMetOnAllServers(b, i, k, todos[k].vc) && AllVersionsInDepsAreMetOnAllServers(b, i, todos[k].deps)
+
+    ensures forall k :: k in res ==> MetaValid(res[k]) && res[k].key == k 
+    ensures forall k :: k in res ==> AVersionIsMetOnAllServers(b, i, k, res[k].vc) && AllVersionsInDepsAreMetOnAllServers(b, i, res[k].deps)
+    decreases |icache.Values|, |deps|
+{
+    reveal_AllVersionsInDepsAreMetOnAllServers();
+    // reveal_AllVersionsInCCacheAreMetOnAllServers();
+    
+    // assert forall k :: k in todos ==> AVersionIsMetOnAllServers(b, i, k, todos[k].vc); //&& AllVersionsInDepsAreMetOnAllServers(b, i, todos[k].deps);
+    if |deps| == 0 then 
+        todos
+    else 
+        var k :| k in deps;
+        var new_deps := RemoveElt(deps, k);
+        if k in todos && (VCHappendsBefore(deps[k], todos[k].vc) || VCEq(deps[k], todos[k].vc)) then 
+            var res := GetMetasOfAllDepsGlobalView3(b, i, idx, vc, icache, new_deps, todos, domain);
+            res
+        else 
+            var metas := set m | m in icache[k] && (VCHappendsBefore(m.vc, deps[k]) || VCEq(m.vc, deps[k]));
+            if |metas| > 0 then
+            
+                var initial := EmptyMeta(k);
+                var merged := FoldMetaSet(initial, metas, domain);
+                var meta := merged.(vc := deps[k]);
+                
+                lemma_FoldMetaBounded(initial, metas, deps[k], domain);
+                assert (VCHappendsBefore(merged.vc, meta.vc) || VCEq(merged.vc, meta.vc));
+
+                var new_cache := icache[k:= icache[k] - metas];
+                assert icache[k] >= metas;
+                lemma_MapRemoveSubsetOfTheValOfKey(icache, k, metas);
+                assert |new_cache.Values| < |icache.Values|;
+
+                assert forall m :: m in metas ==> VCHappendsBefore(m.vc, meta.vc) || VCEq(m.vc, meta.vc);
+                assert VCHappendsBefore(meta.vc, vc) || VCEq(meta.vc, vc);
+                lemma_MetaIsMetImpliesMetasBeforeItAreMet3(b, i, idx, vc, metas);
+                assert forall m :: m in metas ==> AVersionIsMetOnAllServers(b, i, m.key, m.vc);
+                assert forall m :: m in metas ==> AllVersionsInDepsAreMetOnAllServers(b, i, m.deps);
+
+                assert MetaValid(initial);
+                assert forall kk :: kk in initial.deps ==> kk in domain;
+                assert AllVersionsInDepsAreMetOnAllServers(b, i, initial.deps);
+                lemma_FoldMetasPreservesDepsAreMet(b, i, initial, metas, domain);
+                assert AllVersionsInDepsAreMetOnAllServers(b, i, meta.deps);
+
+                var res := GetMetasOfAllDepsGlobalView3(b, i, idx, vc, new_cache, merged.deps, todos, domain);
+
+                assume forall k :: k in res ==> AVersionIsMetOnAllServers(b, i, k, res[k].vc) && AllVersionsInDepsAreMetOnAllServers(b, i, res[k].deps);
+                assume AVersionIsMetOnAllServers(b, i, k, meta.vc);
+
+                var todos' := AddMetaToMetaMap(res, meta);
+
+                assume AllVersionsInDepsAreMetOnAllServers(b, i, new_deps);
+                lemma_MetaMapIsMetImpliesInsertedMataMapIsMet(b, i, res, meta);
+                assume forall k :: k in todos' ==> AVersionIsMetOnAllServers(b, i, k, todos'[k].vc) && AllVersionsInDepsAreMetOnAllServers(b, i, todos'[k].deps);
+
+                var res' := GetMetasOfAllDepsGlobalView3(b, i, idx, vc, icache, new_deps, todos', domain);
+                res'
+            else 
+                var initial := EmptyMeta(k);
+                var meta := initial.(vc:=deps[k]);
+
+                assume AllVersionsInDepsAreMetOnAllServers(b, i, deps);
+                assume forall k :: k in todos ==> AVersionIsMetOnAllServers(b, i, k, todos[k].vc) && AllVersionsInDepsAreMetOnAllServers(b, i, todos[k].deps);
+                assert AVersionIsMetOnAllServers(b, i, meta.key, meta.vc);
+                assert AllVersionsInDepsAreMetOnAllServers(b, i, meta.deps);
+                
+                var todos' := AddMetaToMetaMap(todos, meta);
+                lemma_MetaMapIsMetImpliesInsertedMataMapIsMet(b, i, todos, meta);
+                assert forall k :: k in todos' ==> AVersionIsMetOnAllServers(b, i, k, todos'[k].vc) && AllVersionsInDepsAreMetOnAllServers(b, i, todos'[k].deps);
+                
+                var res := GetMetasOfAllDepsGlobalView3(b, i, idx, vc, icache, new_deps, todos', domain);
+                res
+}
+
+
+
+lemma lemma_VersionsAfterPullDepsAreMetOnAllServers2(
+    b:Behavior<CMState>,
+    i:int,
+    idx:int,
+    vc:VectorClock,
     deps:Dependency
 )
     requires i > 0
@@ -204,8 +450,10 @@ lemma lemma_VersionsAfterPullDepsAreMetOnAllServers(
     requires CMNext(b[i], b[i+1])
     requires 0 <= idx < Nodes
     requires DependencyValid(deps)
+    requires VectorClockValid(vc)
     requires forall j :: 0 < j <= i ==> AllWriteDepsAreMet(b, j)
     requires forall j :: 0 <= j < i ==> ServerNextDoesNotDecreaseVersions(b[j], b[j+1])
+    requires forall k :: k in deps ==> VCHappendsBefore(deps[k], vc) || VCEq(deps[k], vc)
     requires AllVersionsInDepsAreMetOnAllServers(b, i, deps)
     requires AllVersionsInCCacheAreMetOnAllServers(b, i, b[i].servers[idx].s.ccache)
     ensures var res := PullDeps2(b[i].servers[idx].s.icache, b[i].servers[idx].s.ccache, deps);
@@ -222,9 +470,9 @@ lemma lemma_VersionsAfterPullDepsAreMetOnAllServers(
     var domain := icache.Keys + deps.Keys;
 
     var todos := GetMetasOfAllDeps(icache, deps, map[], domain);
-    var todos1 := GetMetasOfAllDepsGlobalView2(b, i, idx, icache, deps, map[], domain);
+    var todos1 := GetMetasOfAllDepsGlobalView3(b, i, idx, vc, icache, deps, map[], domain);
     assert forall k :: k in todos1 ==> AVersionIsMetOnAllServers(b, i, k, todos1[k].vc) && AllVersionsInDepsAreMetOnAllServers(b, i, todos1[k].deps);
-    lemma_GetMetasOfAllDepsGlobalViewEqualsToGetMetasOfAllDeps2(b, i, idx, icache, deps, map[], domain);
+    lemma_GetMetasOfAllDepsGlobalViewEqualsToGetMetasOfAllDeps3(b, i, idx, vc, icache, deps, map[], domain);
     assert todos == todos1;
     assert forall k :: k in todos ==> AVersionIsMetOnAllServers(b, i, k, todos[k].vc) && AllVersionsInDepsAreMetOnAllServers(b, i, todos[k].deps);
 
@@ -237,11 +485,53 @@ lemma lemma_VersionsAfterPullDepsAreMetOnAllServers(
     assert AllVersionsInCCacheAreMetOnAllServers(b, i, res.1);
 }
 
+// lemma lemma_VersionsAfterPullDepsAreMetOnAllServers(
+//     b:Behavior<CMState>,
+//     i:int,
+//     idx:int,
+//     deps:Dependency
+// )
+//     requires i > 0
+//     requires IsValidBehaviorPrefix(b, i)
+//     requires CMNext(b[i], b[i+1])
+//     requires 0 <= idx < Nodes
+//     requires DependencyValid(deps)
+//     requires forall j :: 0 < j <= i ==> AllWriteDepsAreMet(b, j)
+//     requires forall j :: 0 <= j < i ==> ServerNextDoesNotDecreaseVersions(b[j], b[j+1])
+//     requires AllVersionsInDepsAreMetOnAllServers(b, i, deps)
+//     requires AllVersionsInCCacheAreMetOnAllServers(b, i, b[i].servers[idx].s.ccache)
+//     ensures var res := PullDeps2(b[i].servers[idx].s.icache, b[i].servers[idx].s.ccache, deps);
+//             AllVersionsInCCacheAreMetOnAllServers(b, i, res.1)
+// {
+//     lemma_BehaviorValidImpliesOneStepValid(b, i);
+//     reveal_AllVersionsInDepsAreMetOnAllServers();
+//     // reveal_AllDepsInICacheAreMetOnAllServers();
+//     reveal_AllVersionsInCCacheAreMetOnAllServers();
+    
+//     // assert CMNextCommon(b[i-1], b[i]);
+//     var icache := b[i].servers[idx].s.icache;
+//     var ccache := b[i].servers[idx].s.ccache;
+//     var domain := icache.Keys + deps.Keys;
+
+//     var todos := GetMetasOfAllDeps(icache, deps, map[], domain);
+//     var todos1 := GetMetasOfAllDepsGlobalView2(b, i, idx, icache, deps, map[], domain);
+//     assert forall k :: k in todos1 ==> AVersionIsMetOnAllServers(b, i, k, todos1[k].vc) && AllVersionsInDepsAreMetOnAllServers(b, i, todos1[k].deps);
+//     lemma_GetMetasOfAllDepsGlobalViewEqualsToGetMetasOfAllDeps2(b, i, idx, icache, deps, map[], domain);
+//     assert todos == todos1;
+//     assert forall k :: k in todos ==> AVersionIsMetOnAllServers(b, i, k, todos[k].vc) && AllVersionsInDepsAreMetOnAllServers(b, i, todos[k].deps);
+
+//     var new_cache := MergeCCache(ccache, todos);
+//     lemma_MergeCCacheEnsuresAllVersionAreMetOnAllServers(b, i, ccache, todos);
+//     assert AllVersionsInCCacheAreMetOnAllServers(b, i, new_cache);
+
+//     var res := PullDeps2(icache, ccache, deps);
+//     assert res.1 == new_cache;
+//     assert AllVersionsInCCacheAreMetOnAllServers(b, i, res.1);
+// }
 
 
 
-
-lemma {:axiom} lemma_MetaMapIsMetImpliesInsertedMataMapIsMet(
+lemma lemma_MetaMapIsMetImpliesInsertedMataMapIsMet(
     b:Behavior<CMState>,
     i:int,
     todos:map<Key, Meta>,
@@ -251,65 +541,70 @@ lemma {:axiom} lemma_MetaMapIsMetImpliesInsertedMataMapIsMet(
     requires IsValidBehaviorPrefix(b, i)
     requires CMNext(b[i-1], b[i])
     requires forall k :: k in todos ==> MetaValid(todos[k]) && todos[k].key == k 
-                    && forall kk :: kk in todos[k].deps ==> 
-                        VCHappendsBefore(todos[k].deps[kk], todos[k].vc) || VCEq(todos[k].deps[kk], todos[k].vc)
     requires MetaValid(m)
     requires forall k :: k in todos ==> AVersionIsMetOnAllServers(b, i, k, todos[k].vc)  && AllVersionsInDepsAreMetOnAllServers(b, i, todos[k].deps)
     requires AVersionIsMetOnAllServers(b, i, m.key, m.vc) && AllVersionsInDepsAreMetOnAllServers(b, i, m.deps)
     ensures var res := AddMetaToMetaMap(todos, m);
             forall k :: k in res ==> AVersionIsMetOnAllServers(b, i, k, res[k].vc)  && AllVersionsInDepsAreMetOnAllServers(b, i, res[k].deps)
-// {
+{
+    lemma_MetaMapIsMetImpliesInsertedMataMapIsMet1(b, i, todos, m);
+    lemma_MetaMapIsMetImpliesInsertedMataMapIsMet2(b, i, todos, m);
+}
 
-// }
-
-
-
-lemma {:axiom} lemma_FoldMetasPreservesDepsAreMet(
+lemma lemma_MetaMapIsMetImpliesInsertedMataMapIsMet1(
     b:Behavior<CMState>,
     i:int,
-    meta:Meta,
-    metas:set<Meta>,
-    domain:set<Key>
+    todos:map<Key, Meta>,
+    m:Meta
 )
     requires i > 0
     requires IsValidBehaviorPrefix(b, i)
     requires CMNext(b[i-1], b[i])
-    requires MetaValid(meta)
-    requires forall kk :: kk in meta.deps ==> kk in domain
-    requires AllVersionsInDepsAreMetOnAllServers(b, i, meta.deps)
-    requires forall m :: m in metas ==> MetaValid(m) && m.key == meta.key && (forall kk :: kk in m.deps ==> kk in domain) && AllVersionsInDepsAreMetOnAllServers(b, i, m.deps)
-    ensures var res := FoldMetaSet(meta, metas, domain);
-            AllVersionsInDepsAreMetOnAllServers(b, i, res.deps)
-// {
-//     if |metas| == 0 {
-//         var res := FoldMetaSet(meta, metas, domain);
-//         assert res == meta;
-//         assert AllVersionsInDepsAreMetOnAllServers(b, i, res.deps);
-//         return;
-//     }
+    requires forall k :: k in todos ==> MetaValid(todos[k]) && todos[k].key == k 
+    requires MetaValid(m)
+    requires forall k :: k in todos ==> AVersionIsMetOnAllServers(b, i, k, todos[k].vc) // && AllVersionsInDepsAreMetOnAllServers(b, i, todos[k].deps)
+    requires AVersionIsMetOnAllServers(b, i, m.key, m.vc) // && AllVersionsInDepsAreMetOnAllServers(b, i, m.deps)
+    ensures var res := AddMetaToMetaMap(todos, m);
+            forall k :: k in res ==> AVersionIsMetOnAllServers(b, i, k, res[k].vc) // && AllVersionsInDepsAreMetOnAllServers(b, i, res[k].deps)
+{
 
-//     var x :| x in metas;
+}
 
-//     var merged := MetaMerge(meta, x);
-//     var new_metas := metas - {x};
-//     assert AllVersionsInDepsAreMetOnAllServers(b, i, meta.deps);
-//     assert AllVersionsInDepsAreMetOnAllServers(b, i, x.deps);
-//     reveal_AllVersionsInDepsAreMetOnAllServers();
 
-//     assert i > 0;
-//     assert IsValidBehaviorPrefix(b, i);
-//     assert CMNext(b[i-1], b[i]);
-//     assert AllVersionsInDepsAreMetOnAllServers(b, i, merged.deps);
-//     assert MetaValid(merged);
-//     assert forall kk :: kk in merged.deps ==> kk in domain;
-//     assert forall m :: m in new_metas ==> MetaValid(m) && m.key == merged.key && (forall kk :: kk in m.deps ==> kk in domain) && AllVersionsInDepsAreMetOnAllServers(b, i, m.deps);
+lemma lemma_MetaMapIsMetImpliesInsertedMataMapIsMet2(
+    b:Behavior<CMState>,
+    i:int,
+    todos:map<Key, Meta>,
+    m:Meta
+)
+    requires i > 0
+    requires IsValidBehaviorPrefix(b, i)
+    requires CMNext(b[i-1], b[i])
+    requires forall k :: k in todos ==> MetaValid(todos[k]) && todos[k].key == k 
+    requires MetaValid(m)
+    requires forall k :: k in todos ==> AllVersionsInDepsAreMetOnAllServers(b, i, todos[k].deps)
+    requires AllVersionsInDepsAreMetOnAllServers(b, i, m.deps)
+    ensures var res := AddMetaToMetaMap(todos, m);
+            forall k :: k in res ==> AllVersionsInDepsAreMetOnAllServers(b, i, res[k].deps)
+{
+    // reveal_AllVersionsInDepsAreMetOnAllServers();
+    var res := AddMetaToMetaMap(todos, m);
+    if m.key !in todos {
+        assert res == todos[m.key := m];
+        assert forall k :: k in res ==> AllVersionsInDepsAreMetOnAllServers(b, i, res[k].deps);
+    } else {
+        assert res == todos[m.key := MetaMerge(todos[m.key], m)];
+        assert AllVersionsInDepsAreMetOnAllServers(b, i, todos[m.key].deps);
+        assert AllVersionsInDepsAreMetOnAllServers(b, i, m.deps);
+        lemma_MergedDepsIsMetOnAllServers(b, i, todos[m.key].deps, m.deps);
+        assert AllVersionsInDepsAreMetOnAllServers(b, i, DependencyMerge(todos[m.key].deps, m.deps));
+        assert AllVersionsInDepsAreMetOnAllServers(b, i, MetaMerge(todos[m.key], m).deps);
+        assert forall k :: k in res ==> AllVersionsInDepsAreMetOnAllServers(b, i, res[k].deps);
+    }
 
-//     lemma_FoldMetasPreservesDepsAreMet(b, i, merged, new_metas, domain);
-//     assert AllVersionsInDepsAreMetOnAllServers(b, i, FoldMetaSet(merged, new_metas, domain).deps);
-//     // var res := FoldMetaSet(meta, metas, domain);
-//     assert FoldMetaSet(meta, metas, domain) == FoldMetaSet(merged, new_metas, domain);
-//     assert AllVersionsInDepsAreMetOnAllServers(b, i, FoldMetaSet(meta, metas, domain).deps);
-// }
+}
+
+
 
 // function {:opaque} GetMetasOfAllDepsGlobalView(
 //     b:Behavior<CMState>,
@@ -418,117 +713,117 @@ lemma {:axiom} lemma_FoldMetasPreservesDepsAreMet(
 //                 res
 // }
 
-function {:opaque} GetMetasOfAllDepsGlobalView2(
-    b:Behavior<CMState>,
-    i:int,
-    idx:int,
-    icache:ICache,
-    deps:Dependency,
-    todos:map<Key, Meta>,
-    domain:set<Key>
-) : (res:map<Key, Meta>)
-    requires i > 0
-    requires IsValidBehaviorPrefix(b, i)
-    // requires forall j :: 0 <= j < i ==> CMNext(b[j], b[j+1])
-    requires CMNext(b[i-1], b[i])
-    requires 0 <= idx < Nodes
-    // requires icache == b[i].servers[idx].s.icache
-    requires forall k :: k in icache ==> forall m :: m in icache[k] ==> k in b[i].servers[idx].s.icache && m in b[i].servers[idx].s.icache[k]
+// function {:opaque} GetMetasOfAllDepsGlobalView2(
+//     b:Behavior<CMState>,
+//     i:int,
+//     idx:int,
+//     icache:ICache,
+//     deps:Dependency,
+//     todos:map<Key, Meta>,
+//     domain:set<Key>
+// ) : (res:map<Key, Meta>)
+//     requires i > 0
+//     requires IsValidBehaviorPrefix(b, i)
+//     // requires forall j :: 0 <= j < i ==> CMNext(b[j], b[j+1])
+//     requires CMNext(b[i-1], b[i])
+//     requires 0 <= idx < Nodes
+//     // requires icache == b[i].servers[idx].s.icache
+//     requires forall k :: k in icache ==> forall m :: m in icache[k] ==> k in b[i].servers[idx].s.icache && m in b[i].servers[idx].s.icache[k]
 
-    requires forall k :: k in icache ==> k in Keys_domain && (forall m :: m in icache[k] ==> MetaValid(m) && m.key == k
-                && (forall kk :: kk in m.deps ==> kk in domain && kk in Keys_domain))
-    requires DependencyValid(deps)
-    requires forall k :: k in todos ==> MetaValid(todos[k]) && todos[k].key == k 
-    requires forall k :: k in Keys_domain ==> k in icache // should we have this?
-    requires forall k :: k in deps ==> k in domain 
+//     requires forall k :: k in icache ==> k in Keys_domain && (forall m :: m in icache[k] ==> MetaValid(m) && m.key == k
+//                 && (forall kk :: kk in m.deps ==> kk in domain && kk in Keys_domain))
+//     requires DependencyValid(deps)
+//     requires forall k :: k in todos ==> MetaValid(todos[k]) && todos[k].key == k 
+//     requires forall k :: k in Keys_domain ==> k in icache // should we have this?
+//     requires forall k :: k in deps ==> k in domain 
 
-    requires forall j :: 0 < j <= i ==> AllWriteDepsAreMet(b, j)
-    requires forall j :: 0 <= j < i ==> ServerNextDoesNotDecreaseVersions(b[j], b[j+1])
+//     requires forall j :: 0 < j <= i ==> AllWriteDepsAreMet(b, j)
+//     requires forall j :: 0 <= j < i ==> ServerNextDoesNotDecreaseVersions(b[j], b[j+1])
 
-    requires AllVersionsInDepsAreMetOnAllServers(b, i, deps)
-    requires forall k :: k in todos ==> AVersionIsMetOnAllServers(b, i, k, todos[k].vc) && AllVersionsInDepsAreMetOnAllServers(b, i, todos[k].deps)
+//     requires AllVersionsInDepsAreMetOnAllServers(b, i, deps)
+//     requires forall k :: k in todos ==> AVersionIsMetOnAllServers(b, i, k, todos[k].vc) && AllVersionsInDepsAreMetOnAllServers(b, i, todos[k].deps)
 
-    ensures forall k :: k in res ==> MetaValid(res[k]) && res[k].key == k 
-    ensures forall k :: k in res ==> AVersionIsMetOnAllServers(b, i, k, res[k].vc) && AllVersionsInDepsAreMetOnAllServers(b, i, res[k].deps)
-    decreases |icache.Values|, |deps|
-{
-    reveal_AllVersionsInDepsAreMetOnAllServers();
-    // reveal_AllVersionsInCCacheAreMetOnAllServers();
+//     ensures forall k :: k in res ==> MetaValid(res[k]) && res[k].key == k 
+//     ensures forall k :: k in res ==> AVersionIsMetOnAllServers(b, i, k, res[k].vc) && AllVersionsInDepsAreMetOnAllServers(b, i, res[k].deps)
+//     decreases |icache.Values|, |deps|
+// {
+//     reveal_AllVersionsInDepsAreMetOnAllServers();
+//     // reveal_AllVersionsInCCacheAreMetOnAllServers();
     
-    // assert forall k :: k in todos ==> AVersionIsMetOnAllServers(b, i, k, todos[k].vc); //&& AllVersionsInDepsAreMetOnAllServers(b, i, todos[k].deps);
-    if |deps| == 0 then 
-        todos
-    else 
-        var k :| k in deps;
-        var new_deps := RemoveElt(deps, k);
-        if k in todos && (VCHappendsBefore(deps[k], todos[k].vc) || VCEq(deps[k], todos[k].vc)) then 
-            var res := GetMetasOfAllDepsGlobalView2(b, i, idx, icache, new_deps, todos, domain);
-            res
-        else 
-            var metas := set m | m in icache[k] && (VCHappendsBefore(m.vc, deps[k]) || VCEq(m.vc, deps[k]));
-            if |metas| > 0 then
-            // if exists m :: m in icache[k] && VCEq(m.vc, deps[k]) then 
-                var initial := EmptyMeta(k);
-                var merged := FoldMetaSet(initial, metas, domain);
-                var meta := merged.(vc := deps[k]);
-                // var m :| m in icache[k] && VCEq(m.vc, deps[k]);
-                // var meta := m;
+//     // assert forall k :: k in todos ==> AVersionIsMetOnAllServers(b, i, k, todos[k].vc); //&& AllVersionsInDepsAreMetOnAllServers(b, i, todos[k].deps);
+//     if |deps| == 0 then 
+//         todos
+//     else 
+//         var k :| k in deps;
+//         var new_deps := RemoveElt(deps, k);
+//         if k in todos && (VCHappendsBefore(deps[k], todos[k].vc) || VCEq(deps[k], todos[k].vc)) then 
+//             var res := GetMetasOfAllDepsGlobalView2(b, i, idx, icache, new_deps, todos, domain);
+//             res
+//         else 
+//             var metas := set m | m in icache[k] && (VCHappendsBefore(m.vc, deps[k]) || VCEq(m.vc, deps[k]));
+//             if |metas| > 0 then
+//             // if exists m :: m in icache[k] && VCEq(m.vc, deps[k]) then 
+//                 var initial := EmptyMeta(k);
+//                 var merged := FoldMetaSet(initial, metas, domain);
+//                 var meta := merged.(vc := deps[k]);
+//                 // var m :| m in icache[k] && VCEq(m.vc, deps[k]);
+//                 // var meta := m;
                 
-                lemma_FoldMetaBounded(initial, metas, deps[k], domain);
-                assert (VCHappendsBefore(merged.vc, meta.vc) || VCEq(merged.vc, meta.vc));
+//                 lemma_FoldMetaBounded(initial, metas, deps[k], domain);
+//                 assert (VCHappendsBefore(merged.vc, meta.vc) || VCEq(merged.vc, meta.vc));
 
-                var new_cache := icache[k:= icache[k] - metas];
-                assert icache[k] >= metas;
-                lemma_MapRemoveSubsetOfTheValOfKey(icache, k, metas);
-                assert |new_cache.Values| < |icache.Values|;
+//                 var new_cache := icache[k:= icache[k] - metas];
+//                 assert icache[k] >= metas;
+//                 lemma_MapRemoveSubsetOfTheValOfKey(icache, k, metas);
+//                 assert |new_cache.Values| < |icache.Values|;
 
-                assert forall m :: m in metas ==> VCHappendsBefore(m.vc, meta.vc) || VCEq(m.vc, meta.vc);
-                assert forall m :: m in metas ==> m in icache[m.key];
-                assert forall m :: m in metas ==> AVersionOfAKeyIsMet(b[i].servers[idx].s.icache, b[i].servers[idx].s.ccache, m.key, m.vc);
-                assume AVersionIsMetOnAllServers(b, i, meta.key, meta.vc);
-                lemma_MetaIsMetImpliesMetasBeforeItAreMet2(b, i, idx, meta, metas);
-                assert forall m :: m in metas ==> AVersionIsMetOnAllServers(b, i, m.key, m.vc);
-                assert forall m :: m in metas ==> AllVersionsInDepsAreMetOnAllServers(b, i, m.deps);
-                // assume forall j :: 0 <= j < i ==> CMNext(b[j], b[j+1]);
-                // assert MetaValid(meta);
-                // assert forall j :: 0 < j <= i ==> AllWriteDepsAreMet(b, j);
-                // lemma_MetaIsMetImpliesItsDepsAreMet(b, i, meta);
+//                 assert forall m :: m in metas ==> VCHappendsBefore(m.vc, meta.vc) || VCEq(m.vc, meta.vc);
+//                 assert forall m :: m in metas ==> m in icache[m.key];
+//                 assert forall m :: m in metas ==> AVersionOfAKeyIsMet(b[i].servers[idx].s.icache, b[i].servers[idx].s.ccache, m.key, m.vc);
+//                 assume AVersionIsMetOnAllServers(b, i, meta.key, meta.vc);
+//                 lemma_MetaIsMetImpliesMetasBeforeItAreMet2(b, i, idx, meta, metas);
+//                 assert forall m :: m in metas ==> AVersionIsMetOnAllServers(b, i, m.key, m.vc);
+//                 assert forall m :: m in metas ==> AllVersionsInDepsAreMetOnAllServers(b, i, m.deps);
+//                 // assume forall j :: 0 <= j < i ==> CMNext(b[j], b[j+1]);
+//                 // assert MetaValid(meta);
+//                 // assert forall j :: 0 < j <= i ==> AllWriteDepsAreMet(b, j);
+//                 // lemma_MetaIsMetImpliesItsDepsAreMet(b, i, meta);
 
-                assert MetaValid(initial);
-                assert forall kk :: kk in initial.deps ==> kk in domain;
-                assert AllVersionsInDepsAreMetOnAllServers(b, i, initial.deps);
-                lemma_FoldMetasPreservesDepsAreMet(b, i, initial, metas, domain);
-                assert AllVersionsInDepsAreMetOnAllServers(b, i, meta.deps);
+//                 assert MetaValid(initial);
+//                 assert forall kk :: kk in initial.deps ==> kk in domain;
+//                 assert AllVersionsInDepsAreMetOnAllServers(b, i, initial.deps);
+//                 lemma_FoldMetasPreservesDepsAreMet(b, i, initial, metas, domain);
+//                 assert AllVersionsInDepsAreMetOnAllServers(b, i, meta.deps);
 
-                var res := GetMetasOfAllDepsGlobalView2(b, i, idx, new_cache, merged.deps, todos, domain);
+//                 var res := GetMetasOfAllDepsGlobalView2(b, i, idx, new_cache, merged.deps, todos, domain);
 
-                assume forall k :: k in res ==> AVersionIsMetOnAllServers(b, i, k, res[k].vc) && AllVersionsInDepsAreMetOnAllServers(b, i, res[k].deps);
-                assume AVersionIsMetOnAllServers(b, i, k, meta.vc);
+//                 assume forall k :: k in res ==> AVersionIsMetOnAllServers(b, i, k, res[k].vc) && AllVersionsInDepsAreMetOnAllServers(b, i, res[k].deps);
+//                 assume AVersionIsMetOnAllServers(b, i, k, meta.vc);
 
-                var todos' := AddMetaToMetaMap(res, meta);
+//                 var todos' := AddMetaToMetaMap(res, meta);
 
-                assume AllVersionsInDepsAreMetOnAllServers(b, i, new_deps);
-                lemma_MetaMapIsMetImpliesInsertedMataMapIsMet(b, i, res, meta);
-                assume forall k :: k in todos' ==> AVersionIsMetOnAllServers(b, i, k, todos'[k].vc) && AllVersionsInDepsAreMetOnAllServers(b, i, todos'[k].deps);
+//                 assume AllVersionsInDepsAreMetOnAllServers(b, i, new_deps);
+//                 lemma_MetaMapIsMetImpliesInsertedMataMapIsMet(b, i, res, meta);
+//                 assume forall k :: k in todos' ==> AVersionIsMetOnAllServers(b, i, k, todos'[k].vc) && AllVersionsInDepsAreMetOnAllServers(b, i, todos'[k].deps);
 
-                var res' := GetMetasOfAllDepsGlobalView2(b, i, idx, icache, new_deps, todos', domain);
-                res'
-            else 
-                var initial := EmptyMeta(k);
-                var meta := initial.(vc:=deps[k]);
+//                 var res' := GetMetasOfAllDepsGlobalView2(b, i, idx, icache, new_deps, todos', domain);
+//                 res'
+//             else 
+//                 var initial := EmptyMeta(k);
+//                 var meta := initial.(vc:=deps[k]);
 
-                assume AllVersionsInDepsAreMetOnAllServers(b, i, deps);
-                assume forall k :: k in todos ==> AVersionIsMetOnAllServers(b, i, k, todos[k].vc) && AllVersionsInDepsAreMetOnAllServers(b, i, todos[k].deps);
-                assert AVersionIsMetOnAllServers(b, i, meta.key, meta.vc);
-                assert AllVersionsInDepsAreMetOnAllServers(b, i, meta.deps);
+//                 assume AllVersionsInDepsAreMetOnAllServers(b, i, deps);
+//                 assume forall k :: k in todos ==> AVersionIsMetOnAllServers(b, i, k, todos[k].vc) && AllVersionsInDepsAreMetOnAllServers(b, i, todos[k].deps);
+//                 assert AVersionIsMetOnAllServers(b, i, meta.key, meta.vc);
+//                 assert AllVersionsInDepsAreMetOnAllServers(b, i, meta.deps);
                 
-                var todos' := AddMetaToMetaMap(todos, meta);
-                lemma_MetaMapIsMetImpliesInsertedMataMapIsMet(b, i, todos, meta);
-                assert forall k :: k in todos' ==> AVersionIsMetOnAllServers(b, i, k, todos'[k].vc) && AllVersionsInDepsAreMetOnAllServers(b, i, todos'[k].deps);
+//                 var todos' := AddMetaToMetaMap(todos, meta);
+//                 lemma_MetaMapIsMetImpliesInsertedMataMapIsMet(b, i, todos, meta);
+//                 assert forall k :: k in todos' ==> AVersionIsMetOnAllServers(b, i, k, todos'[k].vc) && AllVersionsInDepsAreMetOnAllServers(b, i, todos'[k].deps);
                 
-                var res := GetMetasOfAllDepsGlobalView2(b, i, idx, icache, new_deps, todos', domain);
-                res
-}
+//                 var res := GetMetasOfAllDepsGlobalView2(b, i, idx, icache, new_deps, todos', domain);
+//                 res
+// }
 
 // function GetMetasOfAllDepsGlobalView(
 //     b:Behavior<CMState>,
@@ -732,11 +1027,48 @@ function {:opaque} GetMetasOfAllDepsGlobalView2(
 //             var res2 := GetMetasOfAllDeps(icache, deps, todos, domain);
 //             res1 == res2
 
-lemma {:axiom} lemma_GetMetasOfAllDepsGlobalViewEqualsToGetMetasOfAllDeps2
+// lemma {:axiom} lemma_GetMetasOfAllDepsGlobalViewEqualsToGetMetasOfAllDeps2
+// (
+//     b:Behavior<CMState>,
+//     i:int,
+//     idx:int,
+//     icache:ICache,
+//     deps:Dependency,
+//     todos:map<Key, Meta>,
+//     domain:set<Key>
+// )
+//     requires i > 0
+//     requires IsValidBehaviorPrefix(b, i)
+//     requires CMNext(b[i-1], b[i])
+//     requires 0 <= idx < Nodes
+//     requires icache == b[i].servers[idx].s.icache
+
+//     requires forall k :: k in icache ==> k in Keys_domain && (forall m :: m in icache[k] ==> MetaValid(m) && m.key == k
+//                 && (forall kk :: kk in m.deps ==> kk in domain && kk in Keys_domain))
+//     requires DependencyValid(deps)
+//     requires forall k :: k in todos ==> MetaValid(todos[k]) && todos[k].key == k 
+//     requires forall k :: k in Keys_domain ==> k in icache // should we have this?
+//     requires forall k :: k in deps ==> k in domain 
+
+//     requires forall k :: k in todos ==> forall kk :: kk in todos[k].deps ==> 
+//                         VCHappendsBefore(todos[k].deps[kk], todos[k].vc) || VCEq(todos[k].deps[kk], todos[k].vc)
+//     requires CausalCut(todos)
+
+//     requires forall j :: 0 < j <= i ==> AllWriteDepsAreMet(b, j)
+//     requires forall j :: 0 <= j < i ==> ServerNextDoesNotDecreaseVersions(b[j], b[j+1])
+//     requires AllVersionsInDepsAreMetOnAllServers(b, i, deps)
+//     requires forall k :: k in todos ==> AVersionIsMetOnAllServers(b, i, k, todos[k].vc) && AllVersionsInDepsAreMetOnAllServers(b, i, todos[k].deps)
+//     ensures 
+//             var res1 := GetMetasOfAllDepsGlobalView2(b, i, idx, icache, deps, todos, domain);
+//             var res2 := GetMetasOfAllDeps(icache, deps, todos, domain);
+//             res1 == res2
+
+lemma {:axiom} lemma_GetMetasOfAllDepsGlobalViewEqualsToGetMetasOfAllDeps3
 (
     b:Behavior<CMState>,
     i:int,
     idx:int,
+    vc:VectorClock,
     icache:ICache,
     deps:Dependency,
     todos:map<Key, Meta>,
@@ -746,14 +1078,14 @@ lemma {:axiom} lemma_GetMetasOfAllDepsGlobalViewEqualsToGetMetasOfAllDeps2
     requires IsValidBehaviorPrefix(b, i)
     requires CMNext(b[i-1], b[i])
     requires 0 <= idx < Nodes
-    requires icache == b[i].servers[idx].s.icache
+    requires VectorClockValid(vc)
 
     requires forall k :: k in icache ==> k in Keys_domain && (forall m :: m in icache[k] ==> MetaValid(m) && m.key == k
                 && (forall kk :: kk in m.deps ==> kk in domain && kk in Keys_domain))
     requires DependencyValid(deps)
     requires forall k :: k in todos ==> MetaValid(todos[k]) && todos[k].key == k 
     requires forall k :: k in Keys_domain ==> k in icache // should we have this?
-    requires forall k :: k in deps ==> k in domain 
+    requires forall k :: k in deps ==> k in domain && (VCHappendsBefore(deps[k], vc) || VCEq(deps[k], vc))
 
     requires forall k :: k in todos ==> forall kk :: kk in todos[k].deps ==> 
                         VCHappendsBefore(todos[k].deps[kk], todos[k].vc) || VCEq(todos[k].deps[kk], todos[k].vc)
@@ -764,7 +1096,7 @@ lemma {:axiom} lemma_GetMetasOfAllDepsGlobalViewEqualsToGetMetasOfAllDeps2
     requires AllVersionsInDepsAreMetOnAllServers(b, i, deps)
     requires forall k :: k in todos ==> AVersionIsMetOnAllServers(b, i, k, todos[k].vc) && AllVersionsInDepsAreMetOnAllServers(b, i, todos[k].deps)
     ensures 
-            var res1 := GetMetasOfAllDepsGlobalView2(b, i, idx, icache, deps, todos, domain);
+            var res1 := GetMetasOfAllDepsGlobalView3(b, i, idx, vc, icache, deps, todos, domain);
             var res2 := GetMetasOfAllDeps(icache, deps, todos, domain);
             res1 == res2
 }
