DistributedSystems/VerifiedDS/src/Dafny/Distributed/Protocol/CausalMesh/proof/meta_is_met.dfy
@@ -101,115 +101,115 @@ import opened Collections__Maps2_s
 //     assert AllVersionsInDepsAreMetOnAllServers(b, i, meta.deps);
 // }
 
-lemma lemma_MetaIsMetImpliesItsDepsAreMet2(
-    b:Behavior<CMState>,
-    i:int,
-    idx:int,
-    meta:Meta
-)
-    requires 0 < i 
-    requires IsValidBehaviorPrefix(b, i)
-    requires CMNext(b[i-1], b[i])
-    requires 0 <= idx < Nodes
-    requires MetaValid(meta)
-    requires AVersionOfAKeyIsMet(b[i].servers[idx].s.icache, b[i].servers[idx].s.ccache, meta.key, meta.vc)
-    // requires meta in b[i].servers[idx].s.icache[meta.key]
-    // requires meta != EmptyMeta(meta.key)
-    // requires forall j :: 0 <= j < i ==> CMNext(b[j], b[j+1])
+// lemma lemma_MetaIsMetImpliesItsDepsAreMet2(
+//     b:Behavior<CMState>,
+//     i:int,
+//     idx:int,
+//     meta:Meta
+// )
+//     requires 0 < i 
+//     requires IsValidBehaviorPrefix(b, i)
+//     requires CMNext(b[i-1], b[i])
+//     requires 0 <= idx < Nodes
+//     requires MetaValid(meta)
+//     requires AVersionOfAKeyIsMet(b[i].servers[idx].s.icache, b[i].servers[idx].s.ccache, meta.key, meta.vc)
+//     // requires meta in b[i].servers[idx].s.icache[meta.key]
+//     // requires meta != EmptyMeta(meta.key)
+//     // requires forall j :: 0 <= j < i ==> CMNext(b[j], b[j+1])
     
-    requires AVersionIsMetOnAllServers(b, i, meta.key, meta.vc)
-    requires forall j :: 0 < j <= i ==> AllWriteDepsAreMet(b, j)
-    requires forall j :: 0 <= j < i ==> ServerNextDoesNotDecreaseVersions(b[j], b[j+1])
-    ensures AllVersionsInDepsAreMetOnAllServers(b, i, meta.deps)
-{
-    if i == 0 {
-        return;
-    }
+//     requires AVersionIsMetOnAllServers(b, i, meta.key, meta.vc)
+//     requires forall j :: 0 < j <= i ==> AllWriteDepsAreMet(b, j)
+//     requires forall j :: 0 <= j < i ==> ServerNextDoesNotDecreaseVersions(b[j], b[j+1])
+//     ensures AllVersionsInDepsAreMetOnAllServers(b, i, meta.deps)
+// {
+//     if i == 0 {
+//         return;
+//     }
 
-    if i == 1 {
-        lemma_BehaviorValidImpliesOneStepValid(b, i);
-        assert CMNext(b[i-1], b[i]);
-        lemma_MetaIsMetImpliesItsDepsAreMetForIndexOne2(b, i);
-        // reveal_AllVersionsInDepsAreMetOnAllServers();
-        // assert AllVersionsInDepsAreMetOnAllServers(b, i, meta.deps);
-        assert b[i].servers[idx].s.icache == InitICache();
-        assert b[i].servers[idx].s.ccache == InitCCache();
-        if meta != EmptyMeta(meta.key){
-            if VCHappendsBefore(EmptyMeta(meta.key).vc, meta.vc) {
-                assert meta !in b[i].servers[idx].s.icache[meta.key];
-                assert !(VCHappendsBefore(meta.vc, b[i].servers[idx].s.ccache[meta.key].vc) || VCEq(meta.vc, b[i].servers[idx].s.ccache[meta.key].vc));
-                var m := FoldMetaSet2(b[i].servers[idx].s.ccache[meta.key], b[i].servers[idx].s.icache[meta.key]);
-                assert b[i].servers[idx].s.ccache[meta.key] == EmptyMeta(meta.key);
-                assert forall m :: m in b[i].servers[idx].s.icache[meta.key] ==> m == EmptyMeta(meta.key);
-                lemma_FoldEmptyMetasResultInEmptyMeta(b[i].servers[idx].s.ccache[meta.key], b[i].servers[idx].s.icache[meta.key]);
-                assert m == EmptyMeta(meta.key);
-                assert !AVersionOfAKeyIsMet(b[i].servers[idx].s.icache, b[i].servers[idx].s.ccache, meta.key, meta.vc);
-                assert false;
-            } else {
-                lemma_MetaWithNonEmptyDepsImpliesTheVCLargerThanZero(meta);
-                assert meta !in b[i].servers[idx].s.icache[meta.key];
-                assert !(VCHappendsBefore(meta.vc, b[i].servers[idx].s.ccache[meta.key].vc) || VCEq(meta.vc, b[i].servers[idx].s.ccache[meta.key].vc));
-                var m := FoldMetaSet2(b[i].servers[idx].s.ccache[meta.key], b[i].servers[idx].s.icache[meta.key]);
-                assert b[i].servers[idx].s.ccache[meta.key] == EmptyMeta(meta.key);
-                assert forall m :: m in b[i].servers[idx].s.icache[meta.key] ==> m == EmptyMeta(meta.key);
-                lemma_FoldEmptyMetasResultInEmptyMeta(b[i].servers[idx].s.ccache[meta.key], b[i].servers[idx].s.icache[meta.key]);
-                assert m == EmptyMeta(meta.key);
-                assert !AVersionOfAKeyIsMet(b[i].servers[idx].s.icache, b[i].servers[idx].s.ccache, meta.key, meta.vc);
-                assert false;
-            }
-        } 
-        else {
-            reveal_AllVersionsInDepsAreMetOnAllServers();
-            assert AllVersionsInDepsAreMetOnAllServers(b, i, meta.deps);
-        }
-        return;
-    }
+//     if i == 1 {
+//         lemma_BehaviorValidImpliesOneStepValid(b, i);
+//         assert CMNext(b[i-1], b[i]);
+//         lemma_MetaIsMetImpliesItsDepsAreMetForIndexOne2(b, i);
+//         // reveal_AllVersionsInDepsAreMetOnAllServers();
+//         // assert AllVersionsInDepsAreMetOnAllServers(b, i, meta.deps);
+//         assert b[i].servers[idx].s.icache == InitICache();
+//         assert b[i].servers[idx].s.ccache == InitCCache();
+//         if meta != EmptyMeta(meta.key){
+//             if VCHappendsBefore(EmptyMeta(meta.key).vc, meta.vc) {
+//                 assert meta !in b[i].servers[idx].s.icache[meta.key];
+//                 assert !(VCHappendsBefore(meta.vc, b[i].servers[idx].s.ccache[meta.key].vc) || VCEq(meta.vc, b[i].servers[idx].s.ccache[meta.key].vc));
+//                 var m := FoldMetaSet2(b[i].servers[idx].s.ccache[meta.key], b[i].servers[idx].s.icache[meta.key]);
+//                 assert b[i].servers[idx].s.ccache[meta.key] == EmptyMeta(meta.key);
+//                 assert forall m :: m in b[i].servers[idx].s.icache[meta.key] ==> m == EmptyMeta(meta.key);
+//                 lemma_FoldEmptyMetasResultInEmptyMeta(b[i].servers[idx].s.ccache[meta.key], b[i].servers[idx].s.icache[meta.key]);
+//                 assert m == EmptyMeta(meta.key);
+//                 assert !AVersionOfAKeyIsMet(b[i].servers[idx].s.icache, b[i].servers[idx].s.ccache, meta.key, meta.vc);
+//                 assert false;
+//             } else {
+//                 lemma_MetaWithNonEmptyDepsImpliesTheVCLargerThanZero(meta);
+//                 assert meta !in b[i].servers[idx].s.icache[meta.key];
+//                 assert !(VCHappendsBefore(meta.vc, b[i].servers[idx].s.ccache[meta.key].vc) || VCEq(meta.vc, b[i].servers[idx].s.ccache[meta.key].vc));
+//                 var m := FoldMetaSet2(b[i].servers[idx].s.ccache[meta.key], b[i].servers[idx].s.icache[meta.key]);
+//                 assert b[i].servers[idx].s.ccache[meta.key] == EmptyMeta(meta.key);
+//                 assert forall m :: m in b[i].servers[idx].s.icache[meta.key] ==> m == EmptyMeta(meta.key);
+//                 lemma_FoldEmptyMetasResultInEmptyMeta(b[i].servers[idx].s.ccache[meta.key], b[i].servers[idx].s.icache[meta.key]);
+//                 assert m == EmptyMeta(meta.key);
+//                 assert !AVersionOfAKeyIsMet(b[i].servers[idx].s.icache, b[i].servers[idx].s.ccache, meta.key, meta.vc);
+//                 assert false;
+//             }
+//         } 
+//         else {
+//             reveal_AllVersionsInDepsAreMetOnAllServers();
+//             assert AllVersionsInDepsAreMetOnAllServers(b, i, meta.deps);
+//         }
+//         return;
+//     }
 
-    assert 0 < i - 1;
+//     assert 0 < i - 1;
 
-    lemma_ConstantsAllConsistent(b, i-1);
-    lemma_ConstantsAllConsistent(b, i);
+//     lemma_ConstantsAllConsistent(b, i-1);
+//     lemma_ConstantsAllConsistent(b, i);
 
-    lemma_BehaviorValidImpliesOneStepValid(b, i);
+//     lemma_BehaviorValidImpliesOneStepValid(b, i);
 
-    if AVersionIsMetOnAllServers(b, i-1, meta.key, meta.vc)
-    {
-        // assume meta in b[i-1].servers[idx].s.icache[meta.key];
-        lemma_MetaIsMetImpliesItsDepsAreMet2(b, i-1, idx, meta);
-        assume ServerNextDoesNotDecreaseVersions(b[i-1], b[i]);
-        assert i > 1;
-        assert IsValidBehaviorPrefix(b, i);
-        assert CMNext(b[i-1], b[i]);
-        assert DependencyValid(meta.deps);
-        assume AllVersionsInDepsAreMetOnAllServers(b, i-1, meta.deps);
-        lemma_AllVersionsInDepsAreMetOnAllServersWillAlwaysMet(b, i, meta.deps);
-        return;
-    }
+//     if AVersionIsMetOnAllServers(b, i-1, meta.key, meta.vc)
+//     {
+//         // assume meta in b[i-1].servers[idx].s.icache[meta.key];
+//         lemma_MetaIsMetImpliesItsDepsAreMet2(b, i-1, idx, meta);
+//         assume ServerNextDoesNotDecreaseVersions(b[i-1], b[i]);
+//         assert i > 1;
+//         assert IsValidBehaviorPrefix(b, i);
+//         assert CMNext(b[i-1], b[i]);
+//         assert DependencyValid(meta.deps);
+//         assume AllVersionsInDepsAreMetOnAllServers(b, i-1, meta.deps);
+//         lemma_AllVersionsInDepsAreMetOnAllServersWillAlwaysMet(b, i, meta.deps);
+//         return;
+//     }
 
-    // var ios := lemma_ActionThatChangesServerIsThatServersAction(b, i, )
+//     // var ios := lemma_ActionThatChangesServerIsThatServersAction(b, i, )
     
-    // how to find the node that is the tail of propagation of meta?
+//     // how to find the node that is the tail of propagation of meta?
 
-    var ios:seq<CMIo>;
-    var idx :| 0 <= idx < Nodes;
+//     var ios:seq<CMIo>;
+//     var idx :| 0 <= idx < Nodes;
 
-    assert CMNext(b[i-1], b[i]);
-    assert 0 < i; 
-    assert IsValidBehaviorPrefix(b, i);
-    assert MetaValid(meta);
-    assert 0 <= idx < Nodes;
+//     assert CMNext(b[i-1], b[i]);
+//     assert 0 < i; 
+//     assert IsValidBehaviorPrefix(b, i);
+//     assert MetaValid(meta);
+//     assert 0 <= idx < Nodes;
 
-    lemma_IosIsPropagationTail(b, i, idx, ios, meta);
+//     lemma_IosIsPropagationTail(b, i, idx, ios, meta);
 
-    assert ReceivePropagate(b[i-1].servers[idx].s, b[i].servers[idx].s, ios[0].r, ExtractSentPacketsFromIos(ios));
+//     assert ReceivePropagate(b[i-1].servers[idx].s, b[i].servers[idx].s, ios[0].r, ExtractSentPacketsFromIos(ios));
 
-    var p_pro := ios[0].r;
-    assert p_pro.dst == idx;
+//     var p_pro := ios[0].r;
+//     assert p_pro.dst == idx;
 
-    lemma_PropagationAtTail2(b, i, idx, p_pro, ios);
-    assert AllVersionsInDepsAreMetOnAllServers(b, i, p_pro.msg.meta.deps);
-    assert AllVersionsInDepsAreMetOnAllServers(b, i, meta.deps);
-}
+//     lemma_PropagationAtTail2(b, i, idx, p_pro, ios);
+//     assert AllVersionsInDepsAreMetOnAllServers(b, i, p_pro.msg.meta.deps);
+//     assert AllVersionsInDepsAreMetOnAllServers(b, i, meta.deps);
+// }
 
 // lemma {:axiom} lemma_MetaIsMetImpliesItsDepsAreMetForIndexOne(
 //     b:Behavior<CMState>,
@@ -243,41 +243,78 @@ lemma lemma_MetaIsMetImpliesItsDepsAreMetForIndexOne2(
     assert CMNext(b[i-1], b[i]);
 }
 
-lemma {:axiom} lemma_IosIsPropagationTail(
-    b:Behavior<CMState>,
-    i:int,
-    idx:int,
-    ios:seq<CMIo>,
-    meta:Meta
-)
-    requires 0 < i 
-    requires IsValidBehaviorPrefix(b, i)
-    requires CMNext(b[i-1], b[i])
-    requires MetaValid(meta)
-    requires 0 <= idx < Nodes
-    ensures |ios| > 1
-    ensures ios[0].LIoOpReceive?
-    ensures ios[0].r.msg.Message_Propagation?
-    ensures ios[0].r in b[i-1].environment.sentPackets
-    ensures ReceivePropagate(b[i-1].servers[idx].s, b[i].servers[idx].s, ios[0].r, ExtractSentPacketsFromIos(ios))
-    ensures ios[0].r.msg.start == b[i-1].servers[idx].s.next
-    ensures ios[0].r.msg.round == 2
-    ensures ios[0].r.dst == idx
-    ensures ios[0].r.msg.meta == meta
-    // ensures forall j :: 0 < j <= i ==> AllWriteDepsAreMet(b, j)
+// lemma {:axiom} lemma_IosIsPropagationTail(
+//     b:Behavior<CMState>,
+//     i:int,
+//     idx:int,
+//     ios:seq<CMIo>,
+//     meta:Meta
+// )
+//     requires 0 < i 
+//     requires IsValidBehaviorPrefix(b, i)
+//     requires CMNext(b[i-1], b[i])
+//     requires MetaValid(meta)
+//     requires 0 <= idx < Nodes
+//     ensures |ios| > 1
+//     ensures ios[0].LIoOpReceive?
+//     ensures ios[0].r.msg.Message_Propagation?
+//     ensures ios[0].r in b[i-1].environment.sentPackets
+//     ensures ReceivePropagate(b[i-1].servers[idx].s, b[i].servers[idx].s, ios[0].r, ExtractSentPacketsFromIos(ios))
+//     ensures ios[0].r.msg.start == b[i-1].servers[idx].s.next
+//     ensures ios[0].r.msg.round == 2
+//     ensures ios[0].r.dst == idx
+//     ensures ios[0].r.msg.meta == meta
+//     // ensures forall j :: 0 < j <= i ==> AllWriteDepsAreMet(b, j)
 
-lemma {:axiom} lemma_MetaIsMetImpliesAllPreviousMetasAreMet(
+// lemma {:axiom} lemma_MetaIsMetImpliesAllPreviousMetasAreMet(
+//     b:Behavior<CMState>,
+//     i:int,
+//     meta:Meta,
+//     meta2:Meta
+// )
+//     requires i > 0
+//     requires IsValidBehaviorPrefix(b, i)
+//     requires MetaValid(meta)
+//     requires MetaValid(meta2)
+//     requires AVersionIsMetOnAllServers(b, i, meta.key, meta.vc)
+//     requires VCHappendsBefore(meta2.vc, meta.vc) || VCEq(meta2.vc, meta.vc)
+//     ensures AVersionIsMetOnAllServers(b, i, meta2.key, meta2.vc)
+
+lemma lemma_AVersionIsPropagatedImpliesAllPreviousDepsAreMet(
     b:Behavior<CMState>,
     i:int,
-    meta:Meta,
-    meta2:Meta
+    vc:VectorClock,
+    deps:Dependency
 )
     requires i > 0
     requires IsValidBehaviorPrefix(b, i)
-    requires MetaValid(meta)
-    requires MetaValid(meta2)
-    requires AVersionIsMetOnAllServers(b, i, meta.key, meta.vc)
-    requires VCHappendsBefore(meta2.vc, meta.vc) || VCEq(meta2.vc, meta.vc)
-    ensures AVersionIsMetOnAllServers(b, i, meta2.key, meta2.vc)
-    
+    requires VectorClockValid(vc)
+    requires DependencyValid(deps)
+    requires forall k :: k in deps ==> VCHappendsBefore(deps[k], vc) || VCEq(deps[k], vc)
+    ensures AllVersionsInDepsAreMetOnAllServers(b, i, deps)
+{
+    reveal_AllVersionsInDepsAreMetOnAllServers();
+    forall k | k in deps 
+        ensures AVersionIsMetOnAllServers(b, i, k, deps[k])
+    {
+        assert VCHappendsBefore(deps[k], vc) || VCEq(deps[k], vc);
+        lemma_AVersionIsPropagatedImpliesAllPreviousVersionsAreMet(b, i, vc, k, deps[k]);
+        assert AVersionIsMetOnAllServers(b, i, k, deps[k]);
+    }
+}
+
+lemma {:axiom} lemma_AVersionIsPropagatedImpliesAllPreviousVersionsAreMet(
+    b:Behavior<CMState>,
+    i:int,
+    vc:VectorClock,
+    key:Key,
+    vc2:VectorClock
+)
+    requires i > 0
+    requires IsValidBehaviorPrefix(b, i)
+    requires VectorClockValid(vc2)
+    requires VectorClockValid(vc)
+    requires key in Keys_domain
+    requires VCHappendsBefore(vc2, vc) || VCEq(vc2, vc)
+    ensures AVersionIsMetOnAllServers(b, i, key, vc2)
 }
